Start doing pvec scoping and conversion

theories/autosubst/CCAST.sig
@@ -65,8 +65,8 @@ evnil : cterm -> cterm
 evcons : cterm -> cterm -> cterm
 evec_elim : cterm -> cterm -> cterm -> cterm -> cterm
 
-pvec : cterm -> cterm -> cterm -> cterm -> cterm -> cterm
+pvec : cterm -> cterm -> cterm -> cterm -> cterm
 pvnil : cterm -> cterm
 pvcons : cterm -> cterm -> cterm -> cterm
-pvec_elim : cterm -> cterm -> cterm -> cterm -> cterm -> cterm -> cterm -> cterm -> cterm -> cterm -> cterm -> cterm
+pvec_elim : cterm -> cterm -> cterm -> cterm -> cterm -> cterm -> cterm -> cterm -> cterm -> cterm -> cterm -> cterm -> cterm
 pvec_elimP : cterm -> cterm -> cterm -> cterm -> cterm -> cterm -> cterm -> cterm -> cterm -> cterm -> cterm
